Meta_theory/Models/beeson_to_tarski.v
@@ -7,374 +7,239 @@ Context `{BTn:intuitionistic_Tarski_neutral_dimensionless}.
 
 Lemma cong_stability_eq_stability : forall A B : ITpoint, ~ A <> B -> A = B.
 Proof.
-intros A B HAB.
-apply Icong_identity with A.
-apply Cong_stability.
-intro HNCong.
-apply HAB.
-intro HEq.
-subst.
-apply HNCong.
-apply Icong_pseudo_reflexivity.
+intros A B HAB; apply Icong_identity with A, Cong_stability.
+intro HNC; apply HAB; intro; subst; apply HNC, Icong_pseudo_reflexivity.
 Qed.
 
 End Proof_of_eq_stability_in_IT.
-
-Require Import Classical.
 
 Section Intuitionistic_Tarski_to_Tarski.
 
 Context `{BTn:intuitionistic_Tarski_neutral_dimensionless}.
 
-Lemma col_dec : forall A B C, ICol A B C \/ ~ ICol A B C.
+Variable ED : forall A B : ITpoint, A = B \/ A <> B.
+
+Lemma IT_dec : forall A B C, IT A B C \/ ~ IT A B C.
 Proof.
-intros.
-tauto.
+intros A B C; elim (ED A B); intro HAB; elim (ED B C); intro HBC;
+[left..|]; [intros [HF _]; auto..|intros [_ [HF _]]; auto|].
+destruct (Isegment_construction A B B C HAB) as [D [HB HC]].
+elim (ED C D); intro HCD; [left; subst; auto|].
+right; intro HF; apply HB; clear HB; split; [auto|split; intro HB1].
+
+  {
+  apply HCD, Icong_identity with B; subst.
+  apply Icong_inner_transitivity with D C; [apply Icong_pseudo_reflexivity|].
+  apply Icong_inner_transitivity with D D; [auto|].
+  apply Icong_pseudo_reflexivity.
+  }
+
+  {
+  apply HF; split; [auto|split; [auto|intro HB2]].
+  cut (ICong C C C D); [intro; apply HCD; apply Icong_identity with C;
+                        apply Icong_inner_transitivity with C C;
+                        [auto|apply Icong_pseudo_reflexivity]|].
+  assert (H : forall A B, ICong A B A B).
+    {
+    intros E F; apply Icong_inner_transitivity with F E;
+    apply Icong_pseudo_reflexivity.
+    }
+  apply Ifive_segment with A A B B; auto;
+  [|apply Icong_inner_transitivity with B D; auto].
+  apply Icong_inner_transitivity with D A; [|apply Icong_pseudo_reflexivity].
+  apply Icong_inner_transitivity with C A; [|apply Icong_pseudo_reflexivity].
+  apply Ifive_segment with A A B B; auto; [|intros [_ [_ HNB]]; auto].
+  apply Icong_inner_transitivity with B D; auto.
+  }
 Qed.
 
-Lemma eq_dec : forall A B :ITpoint, A=B \/ A<>B.
+Lemma ICol_dec : forall A B C, ICol A B C \/ ~ ICol A B C.
 Proof.
-intros.
-tauto.
+intros A B C; elim (IT_dec A B C); intro HB1;
+elim (IT_dec A C B); intro HB2; elim (IT_dec C A B); intro HB3;
+[left..|]; [intros [HNB1 [HNB2 HNB3]]; auto..|].
+right; intro HC; apply HC; split; [auto|split; auto].
 Qed.
 
-Definition BetT A B C := IBet A B C \/ A=B \/ B=C.
+Definition BetT A B C := IBet A B C \/ A = B \/ B = C.
 
 Lemma bet_id : forall A B : ITpoint, BetT A B A -> A = B.
 Proof.
-intros.
-unfold BetT in H.
-decompose [or] H.
-apply Ibetween_identity in H0.
-elim H0.
-assumption.
-intuition.
+intros A B [|[|]]; auto; exfalso; apply (Ibetween_identity A B); auto.
 Qed.
 
-Lemma IT_chara : forall A B C,
- IT A B C <-> A=B \/ B=C \/ IBet A B C.
+Lemma IT_chara : forall A B C, IT A B C <-> A = B \/ B = C \/ IBet A B C.
 Proof.
-intros.
-unfold IT.
-tauto. (* classical *)
+intros A B C; split; [|intros [H|[H|H]]; intros [HAB [HBC HB]]; auto].
+intro HB; elim (ED A B); [auto|intro HAB]; elim (ED B C); [auto|intro HBC].
+right; right; apply Bet_stability; intro HNB; apply HB; auto.
+Qed.
+
+Lemma BetT_dec : forall A B C, BetT A B C \/ ~ BetT A B C.
+Proof.
+intros A B C; elim (IT_dec A B C); intro HB; [left|right].
+
+  {
+  unfold BetT; apply IT_chara in HB; tauto.
+  }
+
+  {
+  intros [|[|]]; apply HB, IT_chara; auto.
+  }
+Qed.
+
+Lemma ICol_chara : forall A B C,
+  ICol A B C <-> IT A B C \/ IT B C A \/ IT C A B.
+Proof.
+intros A B C; split.
+
+  {
+  intro HC; elim (IT_dec A B C); intro HB1; [auto|].
+  elim (IT_dec B C A); intro HB2; [auto|].
+  elim (IT_dec C A B); intro HB3; [auto|].
+  exfalso; apply HC; split; [auto|split; [|auto]].
+  intro HNB; apply HB2; intros [HNE1 [HN2 HB]].
+  apply HNB; split; [auto|split; [auto|]].
+  intro; apply HB, Ibetween_symmetry; auto.
+  }
+
+  {
+  intros [|[|]]; intros [HB1 [HB2 HB3]]; auto.
+  apply HB2. intros [HE1 [HE2 HNB]]; apply H; split; [auto|split; [auto|]].
+  intro; apply HNB, Ibetween_symmetry; auto.
+  }
 Qed.
 
 Lemma BetT_symmetry : forall A B C, BetT A B C -> BetT C B A.
-Proof.
-intros.
-unfold BetT in *.
-intuition.
-left.
-apply Ibetween_symmetry.
-assumption.
-Qed.
+Proof. intros A B C [|[|]]; [left; apply Ibetween_symmetry|right..]; auto. Qed.
 
-Lemma BetT_id : forall A B, BetT A B A -> A=B.
-Proof.
-intros.
-unfold BetT in *.
-intuition.
-apply Ibetween_identity in H0.
-elim H0.
-Qed.
-
-(* Lemma 4.1 page 22 *)
+(* Lemma 5.1 page 28 *)
 
 Lemma pasch_col_case : forall A B C P Q : ITpoint,
-        BetT A P C ->
-        BetT B Q C -> ICol A B C -> exists x : ITpoint, BetT P x B /\ BetT Q x A.
+  BetT A P C -> BetT B Q C -> ICol A B C ->
+  exists x, BetT P x B /\ BetT Q x A.
 Proof.
-intros.
-elim (eq_dec A B);intro.
- subst.
- exists B.
- unfold BetT;auto.
-elim (eq_dec A C);intro.
- subst.
- apply BetT_id in H.
- subst.
- exists P.
- unfold BetT;auto.
-elim (eq_dec B C);intro.
- subst.
- apply BetT_id in H0.
- subst.
- exists Q.
- unfold BetT;auto.
-elim (eq_dec B Q);intro.
- subst.
- exists Q.
- unfold BetT;auto.
-elim (eq_dec C Q);intro.
- subst.
- exists P.
- split.
- unfold BetT;auto.
- apply BetT_symmetry.
- auto.
-elim (eq_dec A P);intro.
- subst.
- exists P.
- unfold BetT;auto.
-elim (eq_dec C P);intro.
- subst.
- exists Q.
- split.
- apply BetT_symmetry.
- auto.
- unfold BetT;auto.
+intros A B C P Q HB1 HB2 HC.
+elim (ED A B); intro HAB; [subst; exists B; unfold BetT; auto|].
+elim (ED A C); intro HAC; [subst; apply bet_id in HB1; subst;
+                           exists P; unfold BetT; auto|].
+elim (ED B C); intro HBC; [subst; apply bet_id in HB2; subst;
+                           exists Q; unfold BetT; auto|].
+elim (ED A P); intro HAP; [subst; exists P; unfold BetT; auto|].
+elim (ED P C); intro HPC; [subst; exists Q; split;
+                           [apply BetT_symmetry|unfold BetT]; auto|].
+elim (ED B Q); intro HBQ; [subst; exists Q; unfold BetT; auto|].
+elim (ED Q C); intro HQC; [subst; exists P; split;
+                           [unfold BetT|apply BetT_symmetry]; auto|].
+destruct HB1 as [HB1|[|]]; [|tauto..].
+destruct HB2 as [HB2|[|]]; [|tauto..].
+elim (BetT_dec A C B).
 
-unfold ICol in H1.
-spliter.
-apply not_and_or in H1.
-induction H1.
-apply NNPP in H1.
-unfold IT in *.
-apply not_and_or in H1.
-induction H1.
-apply NNPP in H1.
-subst.
-intuition.
-apply not_and_or in H1.
-induction H1.
-apply NNPP in H1.
-subst.
-intuition.
-apply NNPP in H1.
-exists A.
-split.
-apply Ibetween_symmetry in H1.
-induction H.
-assert (T:=Ibetween_inner_transitivity B A P C H1 H).
-unfold BetT.
-left.
-apply Ibetween_symmetry;auto.
-induction H;subst.
-unfold BetT;auto.
-left.
-apply Ibetween_symmetry;auto.
-unfold BetT;auto.
-apply not_and_or in H1.
-induction H1.
-apply NNPP in H1.
-unfold IT in H1.
-apply not_and_or in H1.
-induction H1.
-apply NNPP in H1.
-subst.
-intuition.
-apply not_and_or in H1.
-induction H1.
-apply NNPP in H1.
-subst.
-intuition.
-apply NNPP in H1.
+  {
+  intros [HB3|[|]]; [exists C|subst; tauto..].
+  split; apply BetT_symmetry; left.
 
-exists C.
+    {
+    apply Ibetween_inner_transitivity with A; apply Ibetween_symmetry; auto.
+    }
 
-unfold BetT in H.
-induction H;induction H0.
-split.
-apply BetT_symmetry.
-left.
+    {
+    apply Ibetween_inner_transitivity with B; [|apply Ibetween_symmetry]; auto.
+    }
+  }
+intro HNB1.
+cut (forall A B P Q, A <> B -> B <> C ->
+                     BetT A B C -> IBet A P C -> IBet B Q C ->
+                     exists x : ITpoint, BetT P x B /\ BetT Q x A).
 
-apply Ibetween_inner_transitivity with A.
-apply Ibetween_symmetry;auto.
-apply Ibetween_symmetry;auto.
-apply BetT_symmetry.
-left.
-apply Ibetween_inner_transitivity with B.
-assumption.
-apply Ibetween_symmetry;auto.
-induction H0;subst;intuition.
-induction H;subst;intuition.
-induction H;subst;intuition.
+  {
+  intro HE.
+  elim (BetT_dec A B C); [intro; destruct (HE A B P Q) as [x []]; auto|].
+  intro HNB2.
+  elim (BetT_dec B A C); [intro; destruct (HE B A Q P) as [x []]; auto|];
+  [exists x; auto|intro HNB3].
+  exfalso; apply HC; split; [|split]; intro HIT;
+  [apply HNB3|apply HNB1|apply HNB2]; left; apply Bet_stability; intro HNIT;
+  apply HIT; split; auto; split; auto.
+  intro; apply HNIT, Ibetween_symmetry; auto.
+  }
 
-apply NNPP in H1.
-induction H;induction H0.
-
-exists B.
-split.
-unfold BetT;auto.
-
-left.
-apply Ibetween_symmetry.
-apply Ibetween_inner_transitivity with C.
-unfold IT in H1.
-apply not_and_or in H1.
-induction H1.
-apply NNPP in H1.
-subst.
-intuition.
-apply not_and_or in H1.
-induction H1.
-apply NNPP in H1.
-subst.
-intuition.
-apply NNPP in H1.
-assumption.
-assumption.
-
-induction H0;subst;intuition.
-induction H;subst;intuition.
-induction H;subst;intuition.
+  {
+  clear dependent A; clear dependent B; clear dependent P; clear dependent Q.
+  intros A B P Q HAB HBC HB1 HB2 HB3.
+  destruct HB1 as [HB1|[|]]; [|subst; tauto..]; clear HAB HBC.
+  exists B; split; [unfold BetT; auto|].
+  apply BetT_symmetry; left; apply Ibetween_inner_transitivity with C; auto.
+  }
 Qed.
 
 Lemma pasch : forall A B C P Q : ITpoint,
-        BetT A P C ->
-        BetT B Q C -> exists x : ITpoint, BetT P x B /\ BetT Q x A.
+  BetT A P C -> BetT B Q C ->
+  exists x, BetT P x B /\ BetT Q x A.
 Proof.
-intros.
-induction (col_dec A B C).
-eapply pasch_col_case;eauto.
-
-unfold BetT in *.
-decompose [or] H;clear H.
-decompose [or] H0;clear H0.
-
-elim (Iinner_pasch A B C P Q H2 H H1).
-intros.
-spliter.
-exists x.
-split.
-tauto.
-tauto.
-
-subst.
-exists Q;auto.
-subst.
-exists P.
-split.
-auto.
-left.
-apply Ibetween_symmetry.
-auto.
-subst.
-exists P;auto.
-subst.
-decompose [or] H0;clear H0.
-exists Q.
-split.
-left.
-apply Ibetween_symmetry.
-auto.
-auto.
-subst.
-exists Q;auto.
-subst.
-exists C;auto.
+intros A B C P Q HB1 HB2.
+elim (ICol_dec A B C); [apply pasch_col_case; auto|intro HNC].
+destruct HB1 as [HB1|[|]]; subst; [|exists P; unfold BetT; auto|];
+[|exists Q; split; [apply BetT_symmetry|unfold BetT]; auto].
+destruct HB2 as [HB2|[|]]; subst; [|exists Q; unfold BetT; auto|];
+[|exists P; split; [unfold BetT|apply BetT_symmetry; left]; auto].
+destruct (Iinner_pasch A B C P Q) as [x [HB3 HB4]];
+[..|exists x; split; left]; auto.
 Qed.
 
-Lemma five_segment:
- forall A A' B B' C C' D D' : ITpoint,
-        ICong A B A' B' ->
-        ICong B C B' C' ->
-        ICong A D A' D' ->
-        ICong B D B' D' ->
-        BetT A B C -> BetT A' B' C' -> A <> B -> ICong C D C' D'.
+Lemma five_segment: forall A A' B B' C C' D D',
+  ICong A B A' B' -> ICong B C B' C' -> ICong A D A' D' -> ICong B D B' D' ->
+  BetT A B C -> BetT A' B' C' -> A <> B ->
+  ICong C D C' D'.
 Proof.
-intros.
-apply Ifive_segment with A A' B B' ;try assumption.
-unfold IT.
-intro.
-spliter.
-unfold BetT in *.
-intuition.
-unfold BetT in *.
-unfold IT.
-intro.
-intuition.
+intros; apply Ifive_segment with A A' B B'; auto;
+intros [HNE1 [HNE2 HB]]; unfold BetT in *; intuition.
 Qed.
 
-Lemma IT_trivial : forall A B, IT A A B.
+Lemma another_point : forall A, exists B : ITpoint, A <> B.
 Proof.
-intros.
-unfold IT.
-intro.
-spliter.
-intuition.
+intro A; assert (T := Ilower_dim).
+elim (ED A beeson_s_axioms.PA); intro HPA; [|exists beeson_s_axioms.PA; auto].
+elim (ED A beeson_s_axioms.PB); intro HPB; [|exists beeson_s_axioms.PB; auto].
+exfalso; destruct T as [_ [_ T]]; apply T; subst; intros [HF _]; auto.
 Qed.
 
-Lemma IT_trivial2 : forall A B, IT A B B.
+Lemma segment_construction : forall A B C D : ITpoint,
+  exists E : ITpoint, BetT A B E /\ ICong B E C D.
 Proof.
-intros.
-unfold IT.
-intro.
-spliter.
-intuition.
-Qed.
+intros A B C D; elim (ED A B); intro HAB.
 
-Lemma another_point : forall A, exists B:ITpoint, A<>B.
-Proof.
-intros.
-assert (T:=Ilower_dim).
-elim (eq_dec A beeson_s_axioms.PA);intro.
-subst.
-elim (eq_dec beeson_s_axioms.PA beeson_s_axioms.PB);intro.
-rewrite <- H in *.
-exfalso.
-apply T.
-apply IT_trivial.
-exists beeson_s_axioms.PB.
-assumption.
-exists beeson_s_axioms.PA.
-assumption.
-Qed.
+  {
+  subst; destruct (another_point B) as [A HAB].
+  destruct (Isegment_construction A B C D) as [E [HB HC]]; [auto|].
+  exists E; split; auto; apply IT_chara in HB; unfold BetT; tauto.
+  }
 
-Lemma segment_construction :
- forall A B C D : ITpoint,
-        exists E : ITpoint, BetT A B E /\ ICong B E C D.
-Proof.
-intros.
-induction (eq_dec A B).
-subst.
-elim (another_point B);intros.
-elim (Isegment_construction x B C D);intros.
-exists x0.
-split.
-unfold BetT.
-intuition.
-intuition.
-intuition.
-elim (Isegment_construction A B C D H).
-intros.
-exists x.
-spliter.
-split;try assumption.
-unfold IT in *.
-unfold BetT.
-tauto.
+  {
+  destruct (Isegment_construction A B C D HAB) as [E [HB HC]].
+  exists E; split; auto; apply IT_chara in HB; unfold BetT; tauto.
+  }
 Qed.
 
 Lemma lower_dim :
-  ~ (BetT beeson_s_axioms.PA beeson_s_axioms.PB beeson_s_axioms.PC \/ 
-     BetT beeson_s_axioms.PB beeson_s_axioms.PC beeson_s_axioms.PA \/ 
+  ~ (BetT beeson_s_axioms.PA beeson_s_axioms.PB beeson_s_axioms.PC \/
+     BetT beeson_s_axioms.PB beeson_s_axioms.PC beeson_s_axioms.PA \/
      BetT beeson_s_axioms.PC beeson_s_axioms.PA beeson_s_axioms.PB).
 Proof.
-assert (T:=Ilower_dim).
-unfold BetT in *.
-unfold ICol in  *.
-unfold IT in *.
+assert (T:=Ilower_dim); unfold BetT, ICol, IT in *.
 firstorder using Ibetween_symmetry.
 Qed.
 
-Lemma eq_dec_points_from_classic : forall A B : ITpoint, A = B \/ A <> B.
-Proof.
-intros.
-apply classic.
-Qed.
-
 Instance IT_to_T : Tarski_neutral_dimensionless.
-exact
-(Build_Tarski_neutral_dimensionless
-   ITpoint BetT ICong
-   Icong_pseudo_reflexivity Icong_inner_transitivity Icong_identity
-   segment_construction five_segment
-   bet_id pasch beeson_s_axioms.PA beeson_s_axioms.PB beeson_s_axioms.PC lower_dim).
+exact (Build_Tarski_neutral_dimensionless
+         ITpoint BetT ICong
+         Icong_pseudo_reflexivity Icong_inner_transitivity Icong_identity
+         segment_construction five_segment bet_id pasch
+         beeson_s_axioms.PA beeson_s_axioms.PB beeson_s_axioms.PC lower_dim).
 Defined.
 
 Instance IT_to_T_PED :
   Tarski_neutral_dimensionless_with_decidable_point_equality IT_to_T.
-Proof. split; apply eq_dec_points_from_classic. Defined.
+Proof. split; apply ED. Defined.
 
 End Intuitionistic_Tarski_to_Tarski.
